progress and restructure

IMLTT/untyped/Substitution.lean
@@ -7,47 +7,97 @@ inductive Subst : Nat → Nat → Type where
   | lift : Subst m n → Subst (m + 1) (n + 1)
   | extend : Subst m n → Tm m → Subst m (n + 1)
 
-def substVar (x : Fin n) (σ : Subst m n) : Tm m :=
+def substitute_var (x : Fin n) (σ : Subst m n) : Tm m :=
   match σ with
   | .weak ρ => weaken x ρ
-  | .shift σ' => shift_tm (substVar x σ')
+  | .shift σ' => shift_tm (substitute_var x σ')
   | .lift σ' =>
     match x with
     | ⟨0, _⟩ => .var (.mk 0 (by simp []))
-    | ⟨x' + 1, h⟩ => shift_tm (substVar (.mk x' (by simp [Nat.lt_of_succ_lt_succ h])) σ')
+    | ⟨x' + 1, h⟩ => shift_tm (substitute_var (.mk x' (by simp [Nat.lt_of_succ_lt_succ h])) σ')
   | .extend σ' t =>
     match x with
     | ⟨0, _⟩ => t
-    | ⟨x' + 1, h⟩ => substVar (.mk x' (Nat.lt_of_succ_lt_succ h)) σ'
+    | ⟨x' + 1, h⟩ => substitute_var (.mk x' (Nat.lt_of_succ_lt_succ h)) σ'
 
-def lift_subst_n (σ : Subst m n) (i : Nat) : Subst (m + i) (n + i) :=
+def lift_subst_n (i : Nat) (σ : Subst m n) : Subst (m + i) (n + i) :=
   match i with
   | 0 => σ
-  | i' + 1 => .lift (lift_subst_n σ i')
+  | i' + 1 => .lift (lift_subst_n i' σ)
 
 def substitute (t : Tm n) (σ : Subst m n) : Tm m :=
   match t with
   | .unit => .unit
   | .empty => .empty
-  | .pi A B => .pi (substitute A σ) (substitute B (lift_subst_n σ 1))
-  | .sigma A B => .sigma (substitute A σ) (substitute B (lift_subst_n σ 1))
+  | .pi A B => .pi (substitute A σ) (substitute B (lift_subst_n 1 σ))
+  | .sigma A B => .sigma (substitute A σ) (substitute B (lift_subst_n 1 σ))
   | .iden A a a' => .iden (substitute A σ) (substitute a σ) (substitute a' σ)
   | .univ => .univ
-  | .var i => substVar i σ
+  | .var i => substitute_var i σ
   | .tt => .tt
-  | .indUnit A b a => .indUnit (substitute A (lift_subst_n σ 1)) (substitute b σ) (substitute a σ)
-  | .indEmpty A b => .indEmpty (substitute A (lift_subst_n σ 1)) (substitute b σ)
-  | .lam A b => .lam (substitute A σ) (substitute b (lift_subst_n σ 1))
+  | .indUnit A b a => .indUnit (substitute A (lift_subst_n 1 σ)) (substitute b σ) (substitute a σ)
+  | .indEmpty A b => .indEmpty (substitute A (lift_subst_n 1 σ)) (substitute b σ)
+  | .lam A b => .lam (substitute A σ) (substitute b (lift_subst_n 1 σ))
   | .app f a => .app (substitute f σ) (substitute a σ)
   | .pairSigma a b => .pairSigma (substitute a σ) (substitute b σ)
-  | .indSigma A B C c p => .indSigma (substitute A σ) (substitute B (lift_subst_n σ 1)) 
-                            (substitute C (lift_subst_n σ 1)) (substitute c (lift_subst_n σ 2))
+  | .indSigma A B C c p => .indSigma (substitute A σ) (substitute B (lift_subst_n 1 σ)) 
+                            (substitute C (lift_subst_n 1 σ)) (substitute c (lift_subst_n 2 σ))
                             (substitute p σ)
   | .refl A a => .refl (substitute A σ) (substitute a σ)
-  | .j A B b a a' p => .j (substitute A σ) (substitute B (lift_subst_n σ 3))
+  | .j A B b a a' p => .j (substitute A σ) (substitute B (lift_subst_n 3 σ))
                         (substitute b σ) (substitute a σ) (substitute a' σ)
                         (substitute p σ)
 
+def comp_substitute_weaken (σ : Subst l m) (ρ : Weak m n) : Subst l n :=
+  match ρ with
+  | .id => σ
+  | .shift ρ' =>
+    match σ with
+    | .weak ξ => .weak (comp_weaken ξ (.shift ρ'))
+    | .shift σ' => .shift (comp_substitute_weaken σ' (.shift ρ'))
+    | .lift σ' => .shift (comp_substitute_weaken σ' ρ')
+    | .extend σ' t => comp_substitute_weaken σ' ρ'
+  | .lift ρ' =>
+    match σ with
+    | .weak ξ => .weak (comp_weaken ξ (.lift ρ'))
+    | .shift σ' => .shift (comp_substitute_weaken σ' (.lift ρ'))
+    | .lift σ' => .lift (comp_substitute_weaken σ' ρ')
+    | .extend σ' t => .extend (comp_substitute_weaken σ' ρ') t
+
+def comp_weaken_substitute (ρ : Weak l m) (σ : Subst m n) : Subst l n :=
+  match ρ with
+  | .id => σ
+  | .shift ρ' =>
+    match σ with
+    | .weak ξ => .weak (comp_weaken (.shift ρ') ξ)
+    | .shift σ' => .shift (comp_weaken_substitute ρ' (.shift σ'))
+    | .lift σ' => .shift (comp_weaken_substitute ρ' (.lift σ'))
+    | .extend σ' t => .shift (.extend (comp_weaken_substitute ρ' σ') (weaken t ρ'))
+  | .lift ρ' =>
+    match σ with
+    | .weak ξ => .weak (comp_weaken (.lift ρ') ξ)
+    | .shift σ' => .shift (comp_weaken_substitute ρ' σ')
+    | .lift σ' => .lift (comp_weaken_substitute ρ' σ')
+    | .extend σ' t => .extend (comp_weaken_substitute (.lift ρ') σ') (weaken t (.lift ρ'))
+
+def comp_substitute_substitute (σ : Subst l m) (σ' : Subst m n) : Subst l n :=
+  match σ' with
+  | .weak ρ' => comp_substitute_weaken σ ρ'
+  | .shift ξ' =>
+    match σ with
+    | .weak ρ => comp_weaken_substitute ρ (.shift ξ')
+    | .shift ξ => .shift (comp_substitute_substitute ξ (.shift ξ'))
+    | .lift ξ => .shift (comp_substitute_substitute ξ ξ')
+    | .extend ξ t => comp_substitute_substitute ξ ξ'
+  | .lift ξ' =>
+    match σ with
+    | .weak ρ => comp_weaken_substitute ρ (.lift ξ')
+    | .shift ξ => .shift (comp_substitute_substitute ξ (.lift ξ'))
+    | .lift ξ => .lift (comp_substitute_substitute ξ ξ')
+    | .extend ξ t => .extend (comp_substitute_substitute ξ ξ') t
+  | .extend ξ' t => .extend (comp_substitute_substitute σ ξ') (substitute t σ)
+
+-- FIXME: congr to above?
 def comp_subst (t : Tm n) (σ : Subst l m) (σ' : Subst m n) : Tm l :=
   substitute (substitute t σ') σ
 
@@ -61,12 +111,6 @@ def subst_weak (t : Tm n) (σ : Subst l m) (ρ : Weak m n) : Tm l :=
 
 def substitute_zero (t : Tm (n + 1)) (a : Tm n) : Tm n :=
   substitute t (.extend (.weak .id) a)
-
-def length_subst : Subst m n →  Nat -- FIXME: better m - n?
-  | .weak ρ => 0
-  | .shift σ => length_subst σ
-  | .lift σ => length_subst σ
-  | .extend σ s => length_subst σ + 1
 
 prefix : 80 "ₛ" => Subst.weak
 prefix:90 "↑ₛ" => Subst.shift
