IMLTT/typed/proofs/admissable/Weakening.lean
@@ -1,0 +1,99 @@
+import IMLTT.untyped.AbstractSyntax
+import IMLTT.untyped.Weakening
+import IMLTT.untyped.Substitution
+import IMLTT.untyped.proofs.Weakening
+
+import IMLTT.typed.JudgmentsAndRules
+import IMLTT.typed.proofs.Recursor
+import IMLTT.typed.proofs.boundary.BoundaryIsCtx
+
+theorem og_weak : HasType Γ (.var i) A → IsType Γ B
+                  → HasType (Γ ⬝ B) (.var (.succ i)) (weaken A (.shift .id)) :=
+  by
+    intro hiA hB
+    match hB with
+    | a => sorry
+
+theorem weakening :
+  (∀ {n : Nat} {Γ : Ctx n}, Γ ctx → ∀ (B A : Tm n), Γ ⬝ A ctx → Γ ⊢ B type 
+    → Γ ⬝ B ⬝ weaken A Weak.id.shift ctx) ∧
+  (∀ {n : Nat} {Γ : Ctx n} {A : Tm n}, Γ ⊢ A type → ∀ (B : Tm n), Γ ⊢ B type 
+    → Γ ⬝ B ⊢ weaken A Weak.id.shift type) ∧
+  (∀ {n : Nat} {Γ : Ctx n} {A a : Tm n}, (Γ ⊢ a ∶ A) → ∀ (B : Tm n), Γ ⊢ B type 
+    → Γ ⬝ B ⊢ weaken a Weak.id.shift ∶ weaken A Weak.id.shift) ∧
+  (∀ {n : Nat} {Γ : Ctx n} {A A' : Tm n}, Γ ⊢ A ≡ A' type → ∀ (B : Tm n), Γ ⊢ B type 
+    → Γ ⬝ B ⊢ weaken A Weak.id.shift ≡ weaken A' Weak.id.shift type) ∧
+  (∀ {n : Nat} {Γ : Ctx n} {A a a' : Tm n}, (Γ ⊢ a ≡ a' ∶ A) → ∀ (B : Tm n), Γ ⊢ B type 
+    → Γ ⬝ B ⊢ weaken a Weak.id.shift ≡ weaken a' Weak.id.shift ∶ weaken A Weak.id.shift) :=
+  by
+    apply judgment_recursor
+      (motive_1 := fun Γ _hiC =>
+        ∀B, ∀ A, Γ ⬝ A ctx → Γ ⊢ B type
+        → Γ ⬝ B ⬝ (weaken A (.shift .id)) ctx)
+      (motive_2 := fun Γ A _hA =>
+        ∀B, Γ ⊢ B type
+        → Γ ⬝ B ⊢ (weaken A (.shift .id)) type)
+      (motive_3 := fun Γ a A haA =>
+        ∀B, Γ ⊢ B type
+        → HasType (Γ ⬝ B) (weaken a (.shift .id)) (weaken A (.shift .id)))
+      (motive_4 := fun Γ A A' _hAA =>
+        ∀B, Γ ⊢ B type
+        → Γ ⬝ B ⊢ (weaken A (.shift .id)) ≡ (weaken A' (.shift .id)) type)
+      (motive_5 := fun Γ a a' A _haaA =>
+        ∀B, Γ ⊢ B type
+        → Γ ⬝ B ⊢ (weaken a (.shift .id)) ≡ (weaken a' (.shift .id)) ∶ (weaken A (.shift .id)))
+    case IsCtxEmpty =>
+      -- ⊢ ∀ (B A : Tm 0), ε ⬝ A ctx → ε ⊢ B type → ε ⬝ B ⬝ (A⌊↑id⌋) ctx
+      intro B A hiA hB
+      apply IsCtx.extend
+      have hiB := IsCtx.extend IsCtx.empty hB
+      have hA := ctx_extr hiA
+      · apply hiB
+      · sorry
+    any_goals sorry
+
+theorem weakening_ctx : IsCtx (Γ ⬝ A) → IsType Γ B
+                        → IsCtx (Γ ⬝ B ⬝ (weaken A (.shift .id))) :=
+  by
+    intro hiCA hB
+    apply And.left weakening
+    · apply ctx_decr hiCA
+    · apply hiCA
+    · apply hB
+
+theorem weakening_type : IsType Γ A → IsType Γ B
+                         → IsType (Γ ⬝ B) (weaken A (.shift .id)) :=
+  by
+    intro hA hB
+    apply And.left (And.right weakening)
+    · apply hA
+    · apply hB
+
+
+theorem weakening_term : HasType Γ a A → IsType Γ B
+                         → HasType (Γ ⬝ B) (weaken a (.shift .id)) 
+                           (weaken A (.shift .id)) :=
+  by
+    intro haA hB
+    apply And.left (And.right (And.right weakening))
+    · apply haA
+    · apply hB
+
+theorem weakening_type_eq : IsEqualType Γ A A' → IsType Γ B
+                            → IsEqualType (Γ ⬝ B) (weaken A (.shift .id)) 
+                              (weaken A' (.shift .id)) :=
+  by
+    intro hAA hB
+    apply And.left (And.right (And.right (And.right weakening)))
+    · apply hAA
+    · apply hB
+
+theorem weakening_term_eq : IsEqualTerm Γ a a' A → IsType Γ B
+                            → IsEqualTerm (Γ ⬝ B) (weaken a (.shift .id)) 
+                              (weaken a' (.shift .id))
+                              (weaken A (.shift .id)) :=
+  by
+    intro haaA hB
+    apply And.right (And.right (And.right (And.right weakening)))
+    · apply haaA
+    · apply hB
