IMLTT/untyped/proofs/Substitution.lean
@@ -1,0 +1,361 @@
+import IMLTT.untyped.AbstractSyntax
+import IMLTT.untyped.Substitution
+import IMLTT.typed.JudgmentsAndRules
+
+theorem substitution_var_lift {σ σ' : Subst m n} :
+    (∀x, substitute (.var x) σ = substitute (.var x) σ')
+    → (∀x, substitute (.var x) (.lift σ) = substitute (.var x) (.lift σ')) :=
+  by
+    intro h x
+    cases x with
+    | mk i hFin =>
+      cases i with
+      | zero =>
+        rfl
+      | succ i' =>
+        apply congrArg shift_tm (h (.mk i' (Nat.lt_of_succ_lt_succ hFin)))
+
+theorem substitution_var_lift_n {σ σ' : Subst m n} :
+    (∀x, substitute (.var x) σ = substitute (.var x) σ')
+    → (∀x, substitute (.var x) (lift_subst_n l σ) = substitute (.var x) (lift_subst_n l σ')) :=
+  by
+    intro h x
+    cases l with
+    | zero =>
+      simp [lift_subst_n]
+      apply h
+    | succ i' =>
+      cases x with
+      | mk i hFin =>
+        cases i with
+        | zero =>
+          rfl
+        | succ i' =>
+          simp [lift_subst_n]
+          apply substitution_var_lift
+          apply substitution_var_lift_n
+          apply h
+
+theorem substitution_var_substitute {σ σ' : Subst m n} :
+    (∀x, substitute (.var x) σ = substitute (.var x) σ')
+    → (∀t, substitute t σ = substitute t σ') :=
+  by
+    intro h t
+    match t with
+    | .unit =>
+      simp [substitute]
+    | .empty =>
+      simp [substitute]
+    | .pi A B =>
+      simp [substitute]
+      apply And.intro
+      · apply substitution_var_substitute h
+      · apply substitution_var_substitute
+        apply substitution_var_lift_n h
+    | .sigma A B =>
+      simp [substitute]
+      apply And.intro
+      · apply substitution_var_substitute h
+      · apply substitution_var_substitute
+        apply substitution_var_lift_n h
+    | .iden A a a' =>
+      simp [substitute]
+      apply And.intro
+      · apply substitution_var_substitute h
+      · apply And.intro
+        · apply substitution_var_substitute h
+        · apply substitution_var_substitute h
+    | .univ =>
+      simp [substitute]
+    | .var x =>
+      apply h
+    | .tt =>
+      simp [substitute]
+    | .indUnit A b a =>
+      simp [substitute]
+      apply And.intro
+      · apply substitution_var_substitute
+        apply substitution_var_lift h
+      · apply And.intro
+        · apply substitution_var_substitute h
+        · apply substitution_var_substitute h
+    | .indEmpty A b =>
+      simp [substitute]
+      apply And.intro
+      · apply substitution_var_substitute
+        apply substitution_var_lift h
+      · apply substitution_var_substitute h
+    | .lam A b => 
+      simp [substitute]
+      apply And.intro
+      · apply substitution_var_substitute h
+      · apply substitution_var_substitute
+        apply substitution_var_lift h
+    | .app f a => 
+      simp [substitute]
+      apply And.intro
+      · apply substitution_var_substitute h
+      · apply substitution_var_substitute h
+    | .pairSigma a b =>
+      simp [substitute]
+      apply And.intro
+      · apply substitution_var_substitute h
+      · apply substitution_var_substitute h
+    | .indSigma A B C c p =>
+      simp [substitute]
+      apply And.intro
+      · apply substitution_var_substitute h
+      · apply And.intro
+        · apply substitution_var_substitute
+          apply substitution_var_lift h
+        · apply And.intro
+          · apply substitution_var_substitute
+            apply substitution_var_lift h
+          · apply And.intro
+            · apply substitution_var_substitute
+              apply substitution_var_lift_n h
+            · apply substitution_var_substitute h
+    | .refl A a =>
+      simp [substitute]
+      apply And.intro
+      · apply substitution_var_substitute h
+      · apply substitution_var_substitute h
+    | .j A B b a a' p => 
+      simp [substitute]
+      apply And.intro
+      · apply substitution_var_substitute h
+      · apply And.intro
+        · apply substitution_var_substitute
+          apply substitution_var_lift_n h
+        · apply And.intro
+          · apply substitution_var_substitute h
+          · apply And.intro
+            · apply substitution_var_substitute h
+            · apply And.intro
+              · apply substitution_var_substitute h
+              · apply substitution_var_substitute h
+
+theorem substitution_var_lift_id {x : Fin (n + 1)} :
+    substitute (.var x) (.lift (.weak .id)) = substitute (.var x) (.weak .id) :=
+  by
+    match x with
+    | .mk i h =>
+      match i with
+      | 0 => rfl
+      | i' + 1 => rfl
+
+theorem substitution_var_lift_n_id {n m : Nat} {x : Fin (n + m)} :
+    substitute (.var x) (lift_subst_n m (.weak .id)) = substitute (.var x) (.weak .id) :=
+  by
+    match m with
+    | 0 => rfl
+    | m' + 1 =>
+      match x with
+      | .mk i h =>
+        match i with
+        | 0 => rfl
+        | i' + 1 =>
+          have h := substitution_var_lift_n_id (n := n) (x := .mk i' (Nat.lt_of_succ_lt_succ h)) 
+          apply congrArg shift_tm h
+
+theorem substitution_id {t : Tm n} :
+    substitute t (.weak .id) = t :=
+  by
+    match t with
+    | .unit =>
+      simp [substitute]
+    | .empty =>
+      simp [substitute]
+    | .pi A B =>
+      simp [substitute]
+      apply And.intro
+      · apply substitution_id
+      · have h := substitution_id (t := B)
+        rw (config := {occs := .pos [2]}) [←h]
+        apply substitution_var_substitute
+        intro x
+        apply substitution_var_lift_n_id
+    | .sigma A B =>
+      simp [substitute]
+      apply And.intro
+      · apply substitution_id
+      · have h := substitution_id (t := B)
+        rw (config := {occs := .pos [2]}) [←h]
+        apply substitution_var_substitute
+        intro x
+        apply substitution_var_lift_n_id
+    | .iden A a a' =>
+      simp [substitute]
+      apply And.intro
+      · apply substitution_id
+      · apply And.intro
+        · apply substitution_id
+        · apply substitution_id
+    | .univ =>
+      simp [substitute]
+    | .var x =>
+      simp [substitute]
+      rfl
+    | .tt =>
+      simp [substitute]
+    | .indUnit A b a =>
+      simp [substitute]
+      apply And.intro
+      · have h := substitution_id (t := A)
+        rw (config := {occs := .pos [2]}) [←h]
+        apply substitution_var_substitute
+        intro x
+        apply substitution_var_lift_n_id
+      · apply And.intro
+        · apply substitution_id
+        · apply substitution_id
+    | .indEmpty A b =>
+      simp [substitute]
+      apply And.intro
+      · have h := substitution_id (t := A)
+        rw (config := {occs := .pos [2]}) [←h]
+        apply substitution_var_substitute
+        intro x
+        apply substitution_var_lift_n_id
+      · apply substitution_id
+    | .lam A b =>
+      simp [substitute]
+      apply And.intro
+      · apply substitution_id
+      · have h := substitution_id (t := b)
+        rw (config := {occs := .pos [2]}) [←h]
+        apply substitution_var_substitute
+        intro x
+        apply substitution_var_lift_n_id
+    | .app f a =>
+      simp [substitute]
+      apply And.intro
+      · apply substitution_id
+      · apply substitution_id
+    | .pairSigma a b =>
+      simp [substitute]
+      apply And.intro
+      · apply substitution_id
+      · apply substitution_id
+    | .indSigma A B C c p =>
+      simp [substitute]
+      apply And.intro
+      · apply substitution_id
+      · apply And.intro
+        · have h := substitution_id (t := B)
+          rw (config := {occs := .pos [2]}) [←h]
+          apply substitution_var_substitute
+          intro x
+          apply substitution_var_lift_n_id
+        · apply And.intro
+          · have h := substitution_id (t := C)
+            rw (config := {occs := .pos [2]}) [←h]
+            apply substitution_var_substitute
+            intro x
+            apply substitution_var_lift_n_id
+          · apply And.intro
+            · have h := substitution_id (t := c)
+              rw (config := {occs := .pos [2]}) [←h]
+              apply substitution_var_substitute
+              intro x
+              apply substitution_var_lift_n_id
+            · apply substitution_id
+    | .refl A a =>
+      simp [substitute]
+      apply And.intro
+      · apply substitution_id
+      · apply substitution_id
+    | .j A B b a a' p =>
+      simp [substitute]
+      apply And.intro
+      · apply substitution_id
+      · apply And.intro
+        · have h := substitution_id (t := B)
+          rw (config := {occs := .pos [2]}) [←h]
+          apply substitution_var_substitute
+          intro x
+          apply substitution_var_lift_n_id
+        · apply And.intro
+          · apply substitution_id
+          · apply And.intro
+            · apply substitution_id
+            · apply And.intro
+              · apply substitution_id
+              · apply substitution_id
+
+theorem substitution_conv_lift_id :
+    ∀x, substitute (.var x) (.weak (.lift (.id : Weak n n))) 
+      = substitute (.var x) (.lift (.weak .id)) :=
+  by
+    intro x
+    simp [substitute]
+    cases x with
+    | mk i h =>
+      cases i with
+      | zero =>
+        rfl
+      | succ i' =>
+        rfl
+
+theorem substitution_lift_id {t : Tm (n + 1)} :
+    substitute t (.weak (.lift .id)) = t :=
+  by
+    have h := substitution_id (t := t)
+    rw (config := {occs := .pos [2]}) [←h]
+    apply substitution_var_substitute
+    intro i
+    rw [←substitution_var_lift_id]
+    apply substitution_conv_lift_id
+
+theorem substitution_lift_comp {t : Tm (n + 1)} :
+    (substitute t (comp_weaken_substitute (.lift ρ) (.lift σ)))
+    = substitute t (.lift (comp_weaken_substitute ρ σ)) :=
+  by
+    simp [comp_weaken_substitute]
+
+
+theorem substitution_var_lift_n_comp {n : Nat} {x : Fin (m + n + 1)} :
+      substitute (.var x) (comp_weaken_substitute (.lift (lift_weak_n n ρ)) (.lift (lift_subst_n n σ)))
+      = substitute (.var x) (.lift (lift_subst_n n (comp_weaken_substitute ρ σ))) :=
+  by
+    match n with
+    | .zero =>
+      match x with
+      | .mk i hFin =>
+        match i with
+        | .zero => rfl
+        | .succ i' =>
+          simp [substitute]
+          simp [comp_weaken_substitute]
+          simp [lift_weak_n]
+          simp [lift_subst_n]
+    | .succ n' =>
+      match x with
+      | .mk i hFin =>
+        match i with
+        | .zero => rfl
+        | .succ i' =>
+          simp [comp_weaken_substitute]
+          simp [substitute]
+          sorry
+ 
+      -- helper1 (1+ n) (x +1) = trans (sym (wk1-wk≡lift-wk1 _ _)) (cong wk1 (helper1 n x))
+      
+-- theorem substitution_var_lift_n {σ σ' : Subst m n} :
+--     (∀x, substitute (.var x) σ = substitute (.var x) σ')
+--     → (∀x, substitute (.var x) (lift_subst_n l σ) = substitute (.var x) (lift_subst_n l σ')) :=
+
+theorem substitution_lift_n_comp (l : Nat) {t : Tm (n + l)} :
+    (substitute t (comp_weaken_substitute (lift_weak_n l ρ) (lift_subst_n l σ)))
+    = substitute t (lift_subst_n l (comp_weaken_substitute ρ σ)) :=
+  by
+    match l with
+    | 0 => 
+      simp [lift_subst_n]
+      simp [lift_weak_n]
+    | l' + 1 =>
+      simp [lift_subst_n]
+      simp [lift_weak_n]
+      apply substitution_var_substitute
+      apply substitution_var_lift_n_comp
+
