IMLTT/untyped/proofs/Weakening.lean
@@ -1,0 +1,547 @@
+import IMLTT.untyped.AbstractSyntax
+import IMLTT.untyped.Weakening
+import IMLTT.untyped.Substitution
+
+theorem weakening_var_lift {ρ ρ' : Weak m n} :
+    (∀x, weaken_var x ρ = weaken_var x ρ')
+    → (∀x, weaken_var x (.lift ρ) = weaken_var x (.lift ρ')) :=
+  by
+    intro h x
+    cases x with
+    | mk i _h =>
+      match i with
+      | 0 => rfl
+      | i' + 1 =>
+        simp [weaken_var]
+        apply h
+
+theorem weakening_var_lift_n {ρ ρ' : Weak m n}:
+    (∀x, weaken_var x ρ = weaken_var x ρ')
+    → (∀j {x: Fin (n + j)}, weaken_var x (lift_weak_n j ρ) = weaken_var x (lift_weak_n j ρ')) :=
+  by
+    intro h x n
+    cases x with
+    | zero =>
+      simp [lift_weak_n]
+      apply h
+    | succ i =>
+      rw [lift_weak_n]
+      apply weakening_var_lift
+      apply weakening_var_lift_n
+      apply h
+
+theorem weakening_var_weaken :
+    (∀ i, weaken_var i ρ = weaken_var i ρ')
+    → (∀ t, weaken t ρ = weaken t ρ') :=
+  by
+    intro h t
+    match t with
+    | .unit =>
+      simp [weaken]
+    | .empty =>
+      simp [weaken]
+    | .pi A B =>
+      simp [weaken]
+      apply And.intro
+      · apply weakening_var_weaken h
+      · apply weakening_var_weaken
+        intro i
+        apply weakening_var_lift_n h
+    | .sigma A B =>
+      simp [weaken]
+      apply And.intro
+      · apply weakening_var_weaken h
+      · apply weakening_var_weaken
+        intro i
+        apply weakening_var_lift_n h
+    | .iden A a a' =>
+      simp [weaken]
+      apply And.intro
+      · apply weakening_var_weaken h
+      · apply And.intro
+        · apply weakening_var_weaken h
+        · apply weakening_var_weaken h
+    | .univ =>
+      simp [weaken]
+    | .var x =>
+      simp [weaken]
+      apply h
+    | .tt =>
+      simp [weaken]
+    | .indUnit A b a =>
+      simp [weaken]
+      apply And.intro
+      · apply weakening_var_weaken
+        apply weakening_var_lift_n
+        apply h
+      · apply And.intro
+        · apply weakening_var_weaken h
+        · apply weakening_var_weaken h
+    | .indEmpty A b =>
+      simp [weaken]
+      apply And.intro
+      · apply weakening_var_weaken
+        apply weakening_var_lift_n h
+      · apply weakening_var_weaken h
+    | .lam A b =>
+      simp [weaken]
+      apply And.intro
+      · apply weakening_var_weaken h
+      · apply weakening_var_weaken
+        apply weakening_var_lift_n h
+    | .app f a =>
+      simp [weaken]
+      apply And.intro
+      · apply weakening_var_weaken h
+      · apply weakening_var_weaken h
+    | .pairSigma a b =>
+      simp [weaken]
+      apply And.intro
+      · apply weakening_var_weaken h
+      · apply weakening_var_weaken h
+    | .indSigma A B C c p =>
+      simp [weaken]
+      apply And.intro
+      · apply weakening_var_weaken h
+      · apply And.intro
+        · apply weakening_var_weaken
+          apply weakening_var_lift_n h
+        · apply And.intro
+          · apply weakening_var_weaken
+            apply weakening_var_lift_n h
+          · apply And.intro
+            · apply weakening_var_weaken
+              apply weakening_var_lift_n h
+            · apply weakening_var_weaken h
+    | .refl A a =>
+      simp [weaken]
+      apply And.intro
+      · apply weakening_var_weaken h
+      · apply weakening_var_weaken h
+    | .j A B b a a' p =>
+      simp [weaken]
+      apply And.intro
+      · apply weakening_var_weaken h
+      · apply And.intro
+        · apply weakening_var_weaken
+          apply weakening_var_lift_n h
+        · apply And.intro
+          · apply weakening_var_weaken h
+          · apply And.intro
+            · apply weakening_var_weaken h
+            · apply And.intro
+              · apply weakening_var_weaken h
+              · apply weakening_var_weaken h
+
+theorem weakening_var_lift_id {n : Nat} {x : Fin (n + 1)} :
+    weaken_var x (.lift .id) = (weaken_var x .id) :=
+  by
+    match x with
+    | .mk i h =>
+      match i with
+      | 0 => rfl
+      | i' + 1 => rfl
+
+theorem weakening_var_lift_n_id {n m : Nat} {x : Fin (n + m)} :
+    weaken_var x (lift_weak_n m .id) = (weaken_var x .id) :=
+  by
+    match m with
+    | 0 => rfl
+    | m' + 1 =>
+      match x with
+      | .mk i h =>
+        match i with
+        | 0 => rfl
+        | i' + 1 =>
+          rw [lift_weak_n]
+          simp [weaken_var]
+          rw [weakening_var_lift_n_id]
+          rfl
+
+theorem weakening_var_id :
+    ∀ {x: Fin n}, weaken_var x .id = x :=
+  by
+    simp [weaken_var]
+
+theorem weakening_id :
+    ∀{t : Tm n}, weaken t .id = t :=
+  by
+    intro t
+    match t with
+    | .unit =>
+      simp [weaken]
+    | .empty =>
+      simp [weaken]
+    | .pi A B =>
+      simp [weaken]
+      apply And.intro
+      · apply weakening_id
+      · have h := weakening_id (t := B)
+        rw (config := {occs := .pos [2]}) [←h]
+        apply weakening_var_weaken
+        intro i
+        apply weakening_var_lift_n_id
+    | .sigma A B =>
+      simp [weaken]
+      apply And.intro
+      · apply weakening_id
+      · have h := weakening_id (t := B)
+        rw (config := {occs := .pos [2]}) [←h]
+        apply weakening_var_weaken
+        intro i
+        apply weakening_var_lift_n_id
+    | .iden A a a' =>
+      simp [weaken]
+      apply And.intro
+      · apply weakening_id
+      · apply And.intro
+        · apply weakening_id
+        · apply weakening_id
+    | .univ =>
+      simp [weaken]
+    | .var x =>
+      simp [weaken]
+      rfl
+    | .tt =>
+      simp [weaken]
+    | .indUnit A b a =>
+      simp [weaken]
+      apply And.intro
+      · have h := weakening_id (t := A)
+        rw (config := {occs := .pos [2]}) [←h]
+        apply weakening_var_weaken
+        intro i
+        apply weakening_var_lift_n_id
+      · apply And.intro
+        · apply weakening_id
+        · apply weakening_id
+    | .indEmpty A b =>
+      simp [weaken]
+      apply And.intro
+      · have h := weakening_id (t := A)
+        rw (config := {occs := .pos [2]}) [←h]
+        apply weakening_var_weaken
+        intro i
+        apply weakening_var_lift_n_id
+      · apply weakening_id
+    | .lam A b =>
+      simp [weaken]
+      apply And.intro
+      · apply weakening_id
+      · have h := weakening_id (t := b)
+        rw (config := {occs := .pos [2]}) [←h]
+        apply weakening_var_weaken
+        intro i
+        apply weakening_var_lift_n_id
+    | .app f a =>
+      simp [weaken]
+      apply And.intro
+      · apply weakening_id
+      · apply weakening_id
+    | .pairSigma a b => 
+      simp [weaken]
+      apply And.intro
+      · apply weakening_id
+      · apply weakening_id
+    | .indSigma A B C c p =>
+      simp [weaken]
+      apply And.intro
+      · apply weakening_id
+      · apply And.intro
+        · have h := weakening_id (t := B)
+          rw (config := {occs := .pos [2]}) [←h]
+          apply weakening_var_weaken
+          intro i
+          apply weakening_var_lift_n_id
+        · apply And.intro
+          · have h := weakening_id (t := C)
+            rw (config := {occs := .pos [2]}) [←h]
+            apply weakening_var_weaken
+            intro i
+            apply weakening_var_lift_n_id
+          · apply And.intro
+            · have h := weakening_id (t := c)
+              rw (config := {occs := .pos [2]}) [←h]
+              apply weakening_var_weaken
+              intro i
+              apply weakening_var_lift_n_id
+            · apply weakening_id
+    | .refl A a => 
+      simp [weaken]
+      apply And.intro
+      · apply weakening_id
+      · apply weakening_id
+    | .j A B b a a' p =>
+      simp [weaken]
+      apply And.intro
+      · apply weakening_id
+      · apply And.intro
+        · have h := weakening_id (t := B)
+          rw (config := {occs := .pos [2]}) [←h]
+          apply weakening_var_weaken
+          intro i
+          apply weakening_var_lift_n_id
+        · apply And.intro
+          · apply weakening_id
+          · apply And.intro
+            · apply weakening_id
+            · apply And.intro
+              · apply weakening_id
+              · apply weakening_id
+
+theorem weakening_lift_id {t : Tm (n + 1)} : 
+    weaken t (.lift .id) = t :=
+  by
+    have h :=  weakening_id (t := t)
+    rw (config := {occs := .pos [2]}) [←h]
+    apply weakening_var_weaken
+    intro i
+    apply weakening_var_lift_id
+
+theorem weakening_var_comp {ρ : Weak l m} {ρ' : Weak m n} {x : Fin n} :
+    weaken_var (weaken_var x ρ') ρ = weaken_var x (comp_weaken ρ ρ') :=
+  by
+    induction ρ with
+    | id =>
+      simp [weaken_var]
+      rfl
+    | shift γ ih =>
+      rw [comp_weaken]
+      simp [weaken_var]
+      rw [←ih]
+    | lift γ ih =>
+      cases ρ' with
+      | id =>
+        simp [weaken_var]
+      | shift γ' =>
+        rw [comp_weaken]
+        simp [weaken_var]
+        rw [←ih]
+        rfl
+      | lift γ' =>
+        cases x with
+        | mk i hFin =>
+          cases i with
+          | zero => rfl
+          | succ i' =>
+            rw [comp_weaken]
+            simp [weaken_var]
+            rw [←weakening_var_comp]
+            rfl
+
+theorem weakening_comp {ρ : Weak l m} {ρ' : Weak m n} {t : Tm n} :
+    weaken (weaken t ρ') ρ = weaken t (comp_weaken ρ ρ') :=
+  by
+    match t with
+    | .unit =>
+      rfl
+    | .empty =>
+      rfl
+    | .pi A B =>
+      simp [weaken]
+      apply And.intro
+      · apply weakening_comp
+      · apply weakening_comp
+    | .sigma A B =>
+      simp [weaken]
+      apply And.intro
+      · apply weakening_comp
+      · apply weakening_comp
+    | .iden A a a' => 
+      simp [weaken]
+      apply And.intro
+      · apply weakening_comp
+      · apply And.intro
+        · apply weakening_comp
+        · apply weakening_comp
+    | .univ =>
+      rfl
+    | .var x =>
+      simp [weaken]
+      simp [←weakening_var_comp]
+    | .tt =>
+      rfl
+    | .indUnit A b a =>
+      simp [weaken]
+      apply And.intro
+      · apply weakening_comp
+      · apply And.intro
+        · apply weakening_comp
+        · apply weakening_comp
+    | .indEmpty A b =>
+      simp [weaken]
+      apply And.intro
+      · apply weakening_comp
+      · apply weakening_comp
+    | .lam A b =>
+      simp [weaken]
+      apply And.intro
+      · apply weakening_comp
+      · apply weakening_comp
+    | .app f a =>
+      simp [weaken]
+      apply And.intro
+      · apply weakening_comp
+      · apply weakening_comp
+    | .pairSigma a b =>
+      simp [weaken]
+      apply And.intro
+      · apply weakening_comp
+      · apply weakening_comp
+    | .indSigma A B C c p =>
+      simp [weaken]
+      apply And.intro
+      · apply weakening_comp
+      · apply And.intro
+        · apply weakening_comp
+        · apply And.intro
+          · apply weakening_comp
+          · apply And.intro
+            · apply weakening_comp
+            · apply weakening_comp
+    | .refl A a =>
+      simp [weaken]
+      apply And.intro
+      · apply weakening_comp
+      · apply weakening_comp
+    | .j A B b a a' p =>
+      simp [weaken]
+      apply And.intro
+      · apply weakening_comp
+      · apply And.intro
+        · apply weakening_comp
+        · apply And.intro
+          · apply weakening_comp
+          · apply And.intro
+            · apply weakening_comp
+            · apply And.intro
+              · apply weakening_comp
+              · apply weakening_comp
+
+theorem weakening_lift_shift_comp {ρ : Weak m n} :
+    comp_weaken (.shift .id) ρ = comp_weaken (.lift ρ) (.shift .id) :=
+  by
+    match ρ with
+    | .id =>
+      rfl
+    | .shift ρ' =>
+      apply congrArg Weak.shift (weakening_lift_shift_comp (ρ := ρ'))
+    | .lift ρ' =>
+      rfl
+
+theorem weakening_shift_id {ρ : Weak m n} {t : Tm n} :
+    weaken (weaken t ρ) (.shift .id) = weaken t (.shift ρ) :=
+  by
+    apply weakening_comp
+
+theorem weakening_shift_id_lift {ρ : Weak m n} {t : Tm n} :
+    weaken (weaken t (.shift .id)) (.lift ρ) = weaken t (.shift ρ) :=
+  by
+    rw [weakening_comp]
+    rw [←weakening_lift_shift_comp]
+    rfl
+
+theorem weakening_shift_id_outside {ρ : Weak m n} {t : Tm n} :
+    weaken (weaken t ρ) (.shift .id) = weaken (weaken t (.shift .id)) (.lift ρ) :=
+  by
+    rw [weakening_shift_id_lift]
+    rw [weakening_comp]
+    simp [comp_weaken]
+
+-- other (lemmatas needed in some proof)
+
+#reduce ((Tm.pi : Tm 1 → Tm 2 → Tm 1) v(0) v(1))⌊.shift .id⌋
+#reduce ((Tm.pi : Tm 1 → Tm 2 → Tm 1) v(0) v(1))⌊.shift (.shift .id)⌋
+#reduce ((Tm.pi : Tm 1 → Tm 2 → Tm 1) v(0) v(1))⌊(.shift .id)⌋⌊.shift .id⌋
+#reduce ((Tm.refl : Tm 1 → Tm 1 → Tm 1) v(0) v(1))⌊.shift .id⌋
+#reduce ((Tm.refl : Tm 1 → Tm 1 → Tm 1) v(0) v(1))⌊.shift (.shift .id)⌋
+#reduce ((Tm.refl : Tm 1 → Tm 1 → Tm 1) v(0) v(1))⌊.shift .id⌋⌊.shift .id⌋
+
+-- FIXME: lemma is wrong! see .var case
+
+-- theorem weakening_lift_shift {S : Tm (n + 1)} {ρ : Weak m n} :
+--     S⌊.lift (.shift ρ)⌋ = S⌊.lift ρ⌋⌊.lift (.shift .id)⌋ :=
+--   by
+--     match S with
+--     | .unit => 
+--       simp [weaken]
+--     | .empty => 
+--       simp [weaken]
+--     | .pi A B => 
+--       simp [weaken]
+--       apply And.intro
+--       · apply weakening_lift_shift
+--       · simp [lift_weak_n]
+--         rw [weakening_comp]
+--         apply weakening_var_weaken
+--         simp [weaken_var]
+--         intro i
+--         rfl
+--     | .sigma A B =>
+--       simp [weaken]
+--       apply And.intro
+--       · apply weakening_lift_shift
+--       · simp [lift_weak_n]
+--         rw [weakening_comp]
+--         apply weakening_var_weaken
+--         simp [weaken_var]
+--         intro i
+--         rfl
+--     | .iden A a a' =>
+--       simp [weaken]
+--       apply And.intro
+--       · apply weakening_lift_shift
+--       · apply And.intro
+--         · apply weakening_lift_shift
+--         · apply weakening_lift_shift
+--     | .univ =>
+--       simp [weaken]
+--     | .var i =>
+--       simp [weaken]
+--       simp [weaken_var]
+--       match i with
+--       | .mk i' hFin =>
+--         match i' with
+--         | .zero => rfl
+--         | .succ j =>
+--           simp []
+--           sorry
+--       -- match i with
+--       -- | ⟨0, _⟩ => sorry
+--       -- | ⟨x' + 1, h⟩ => sorry
+--     | .tt =>
+--       simp [weaken]
+--     | .indUnit A b a =>
+--       simp [weaken]
+--       simp [lift_weak_n]
+--       sorry
+--     | .indEmpty A b =>
+--       simp [weaken]
+--       simp [lift_weak_n]
+--       sorry
+--     | .lam A b =>
+--       simp [weaken]
+--       simp [lift_weak_n]
+--       sorry
+--     | .app f a => sorry
+--     | .pairSigma a b => sorry
+--     | .indSigma A B C c p =>
+--       simp [weaken]
+--       simp [lift_weak_n]
+--       sorry
+--     | .refl A a => sorry
+--     | .j A B b a a' p =>
+--       simp [weaken]
+--       simp [lift_weak_n]
+--       sorry
+
+theorem weakening_shift_double {S : Tm n} {ρ : Weak m n} : 
+    S⌊.shift (.shift ρ)⌋ = S⌊.shift ρ⌋⌊.shift .id⌋ :=
+  by
+    rw [←weakening_shift_id]
+
+theorem weakening_comp_shift {S : Tm n} {ρ : Weak m n} :
+    S⌊.shift .id ∘ ρ⌋ = S⌊ρ⌋⌊.shift .id⌋ :=
+  by
+    simp [comp_weaken]
+    apply (Eq.symm weakening_shift_id)
